Foam/Seat/Group.lean
@@ -2,28 +2,28 @@ import Foam.Seat
 
 namespace Foam
 
-class Ty06 (G : Type) extends Mul G, One G where
-  d046       : G → G
-  t144   : ∀ a : G, 1 * a = a
-  t143   : ∀ a : G, a * 1 = a
-  t141 : ∀ a b c : G, a * b * c = a * (b * c)
-  t142   : ∀ a : G, a * d046 a = 1
-  t140   : ∀ a : G, d046 a * a = 1
+class Grp (G : Type) extends Mul G, One G where
+  inv       : G → G
+  one_mul   : ∀ a : G, 1 * a = a
+  mul_one   : ∀ a : G, a * 1 = a
+  mul_assoc : ∀ a b c : G, a * b * c = a * (b * c)
+  mul_inv   : ∀ a : G, a * inv a = 1
+  inv_mul   : ∀ a : G, inv a * a = 1
 
-def Ty16.d181 (G : Type) [Ty06 G] : Ty16 G where
-  Ty24     := G
-  d131     := fun g x => g * x
-  t241 := fun x => Foam.Ty06.t144 x
-  t239 := fun g h x => Foam.Ty06.t141 g h x
-  d133     := fun a b => a * Foam.Ty06.d046 b
-  t237 := fun p q => by
-    show (q * Foam.Ty06.d046 p) * p = q
-    rw [Foam.Ty06.t141, Foam.Ty06.t140, Foam.Ty06.t143]
-  t249 := fun g p => by
-    show (g * p) * Foam.Ty06.d046 p = g
-    rw [Foam.Ty06.t141, Foam.Ty06.t142, Foam.Ty06.t143]
+def Seat.principal (G : Type) [Grp G] : Seat G where
+  Pos     := G
+  act     := fun g x => g * x
+  one_act := fun x => Grp.one_mul x
+  mul_act := fun g h x => Grp.mul_assoc g h x
+  sub     := fun a b => a * Grp.inv b
+  act_sub := fun p q => by
+    show (q * Grp.inv p) * p = q
+    rw [Grp.mul_assoc, Grp.inv_mul, Grp.mul_one]
+  sub_act := fun g p => by
+    show (g * p) * Grp.inv p = g
+    rw [Grp.mul_assoc, Grp.mul_inv, Grp.mul_one]
 
-/-- info: 'Foam.Ty16.d181' does not depend on any axioms -/
-#guard_msgs in #print axioms Foam.Ty16.d181
+/-- info: 'Foam.Seat.principal' does not depend on any axioms -/
+#guard_msgs in #print axioms Seat.principal
 
 end Foam
